Simplify Path.Child.class
Add presentation outline

Runtime/Network/Graph/Path/Child.lean
@@ -4,29 +4,25 @@ namespace Network.Graph.Path
 
 def Child (path : Path graph start) := { child // child ≻ path }
 
-theorem Child.parent_eq_nil_class {path : Path graph start} {child : Child path} : (child.val = cons c nil) → start = path.class := by
+namespace Child
+
+theorem parent_eq_nil_class {path : Path graph start} {child : Child path} : (child.val = cons c nil) → start = path.class := by
   intro h
   have h' := child.property
   simp [Succ, h, prefix?] at h'
   simp [←h']
 
--- An extended path's class is a child class of its parent's class.
-def Child.class : (child : Child path) → Class.Child path.class := fun child =>
-  match h : child.val with 
-  | nil => by have := h ▸ child.property.isCons; contradiction
-  | cons c nil => (parent_eq_nil_class h) ▸ c
-  | cons c subpath@(cons _ _) =>
-    have path_isCons := (h ▸ child.property).isCons'
-    have h₁ : c.class = path.snd path_isCons := sorry -- TODO: look at the picture in your folder
-    let pathSuffix := path.suffix path_isCons
-    let subpath := h₁ ▸ subpath
-    have h₂ : subpath ≻ pathSuffix := sorry
-    suffix_class ▸ «class» ⟨subpath, h₂⟩
-termination_by «class» child => sizeOf child.val -- TODO: Perhaps use an explictly define path length property instead.
-decreasing_by sorry
-
-@[simp]
-theorem Child.class_eq_class {child : Child path} : child.class.class = child.val.class := by
+-- TODO: This could also be expressed in `Subpaths.lean` using `prefix?`.
+theorem split_fst_eq_parent (child : Child path) :
+  (child.val.split child.property.isCons).fst = path := by
   sorry
 
+def «class» (child : Child path) : Class.Child path.class :=
+  split_fst_eq_parent child ▸ (child.val.split child.property.isCons).snd
+
+@[simp]
+theorem class_eq_class {child : Child path} : child.class.class = child.val.class := by
+  sorry
+
+end Child
 end Network.Graph.Path
